secure_api/box/experimental_box/Box.ODH_proof/Box.ODH.fsti
@@ -11,7 +11,7 @@ open FStar.Endianness
 
 module MM = FStar.Monotonic.Map
 
-assume val random_bytes: n:nat{n<=32} -> lbytes n
+val random_bytes: n:nat{n<=32} -> lbytes n
 
 noeq type odh_parameters =
   | OP:
@@ -36,53 +36,30 @@ abstract type exponent (oparam:odh_parameters) =
   exponent oparam
 
 val sh_hon: #oparams:odh_parameters -> sh:share oparams -> GTot (b:bool{b=sh.h})
-let sh_hon #oparams sh = sh.h
 
 val exp_hon: #oparams:odh_parameters -> exp:exponent oparams -> GTot (b:bool{b=exp.sh.h})
-let exp_hon #oparams exp = exp.sh.h
 
 val get_exp_share: #oparams:odh_parameters -> e:exponent oparams -> sh:share oparams{e.sh = sh}
-let get_exp_share #oparams e = e.sh
 
 val get_share_raw: #oparams:odh_parameters -> sh:share oparams -> raw:lbytes oparams.share_length{raw = sh.raw_sh}
-let get_share_raw #oparams sh = sh.raw_sh
 
-let gen_dh (oparam:odh_parameters) =
-  let raw_exp = random_bytes oparam.exponent_length in
-  let raw_sh = oparam.exponentiate raw_exp oparam.generator in
-  let sh = SH raw_sh true in
-  EXP raw_exp sh
+val get_exponent_raw: #oparams:odh_parameters -> exp:exponent oparams -> GTot (raw:lbytes oparams.exponent_length{raw = exp.raw_exp})
 
-let coerce_dh_sh  (oparam:odh_parameters) (raw_sh:lbytes oparam.share_length) =
-  SH raw_sh false
+val gen_dh: (oparam:odh_parameters) -> exponent oparam
 
-let coerce_dh_exp  (oparam:odh_parameters) (raw_exp:lbytes oparam.exponent_length) =
-  let raw_sh = oparam.exponentiate raw_exp oparam.generator in
-  let sh = SH raw_sh false in
-  EXP raw_exp sh
+val coerce_dh_sh: (oparam:odh_parameters) -> (rash_sh:lbytes oparam.share_length) -> sh:share oparam
+
+val coerce_dh_exp: (oparam:odh_parameters) -> (raw_exp:lbytes oparam.exponent_length) -> exp:exponent oparam
 
 let id = id:(bytes*bytes)
 
 val create_id: (#oparam:odh_parameters) -> sh1:share oparam -> sh2:share oparam{sh1.raw_sh <> sh2.raw_sh} -> i:id
-let create_id #oparam sh1 sh2 =
-  let int_sh1 = little_endian sh1.raw_sh in
-  let int_sh2 = little_endian sh2.raw_sh in
-  //let int_sh1 = int_of_bytes sh1.raw_sh in
-  //let int_sh2 = int_of_bytes sh2.raw_sh in
-  if int_sh1 < int_sh2 then
-    (sh1.raw_sh,sh2.raw_sh)
-  else
-    (sh2.raw_sh,sh1.raw_sh)
 
 #set-options "--z3rlimit 300 --max_ifuel 0 --max_fuel 1"
 val lemma_symmetric_id: (#oparam:odh_parameters) -> sh1:share oparam -> sh2:share oparam{sh1.raw_sh <> sh2.raw_sh} -> Lemma
   (requires True)
   (ensures create_id sh1 sh2 = create_id sh2 sh1)
   [SMTPat (create_id #oparam sh1 sh2)]
-let lemma_symmetric_id #oparam sh1 sh2 =
-  lemma_little_endian_bij sh1.raw_sh sh2.raw_sh
-  //bytes_of_int_of_bytes sh1.raw_sh;
-  //bytes_of_int_of_bytes sh2.raw_sh
 
 let key_package_log_key = id
 let key_package_log_value (i:id) (key_type:(id -> Type0)) = key_type i
@@ -92,10 +69,9 @@ let key_package_log_inv (key_type:(id -> Type0)) (f:MM.map' (key_package_log_key
 let key_package_log (rgn:erid) (key_type:(id -> Type0)) =
   MM.t rgn (key_package_log_key) (key_package_log_range key_type) (key_package_log_inv key_type)
 
-assume val b:bool
+val b:bool
 
 val get_flag: unit -> GTot (flag:bool{flag = b})
-let get_flag() = b
 
 noeq abstract type odh_package (#key_length:(n:nat{n<=32})) (#key_type:(id -> Type0)) (kp:key_package key_length key_type) (oparam:odh_parameters{oparam.hash_length = key_length}) =
   | ODH:
@@ -104,11 +80,15 @@ noeq abstract type odh_package (#key_length:(n:nat{n<=32})) (#key_type:(id -> Ty
   odh_package #key_length #key_type kp oparam
 
 val get_op_rgn: (#key_length:(n:nat{n<=32})) -> (#key_type:(id -> Type0)) -> (#kp:key_package key_length key_type) -> (#oparam:odh_parameters{oparam.hash_length = key_length}) -> (op:odh_package #key_length #key_type kp oparam) -> (rgn:erid{rgn = op.rgn})
-let get_op_rgn (#key_length:(n:nat{n<=32})) (#key_type:(id -> Type0)) (#kp:key_package key_length key_type) (#oparam:odh_parameters{oparam.hash_length = key_length}) (op:odh_package #key_length #key_type kp oparam) = op.rgn
 
 val get_op_log: (#key_length:(n:nat{n<=32})) -> (#key_type:(id -> Type0)) -> (#kp:key_package key_length key_type) -> (#oparam:odh_parameters{oparam.hash_length = key_length}) -> (op:odh_package #key_length #key_type kp oparam) -> GTot (log:key_package_log op.rgn key_type)
-let get_op_log (#key_length:(n:nat{n<=32})) (#key_type:(id -> Type0)) (#kp:key_package key_length key_type) (#oparam:odh_parameters{oparam.hash_length = key_length}) (op:odh_package #key_length #key_type kp oparam) = op.kp_log
 
+val recall_op_log: (#key_length:(n:nat{n<=32})) -> (#key_type:(id -> Type0)) -> (#kp:key_package key_length key_type) -> (#oparam:odh_parameters{oparam.hash_length = key_length}) -> (op:odh_package #key_length #key_type kp oparam) -> ST unit
+  (requires (fun h0 -> True))
+  (ensures (fun h0 _ h1 ->
+    h0 == h1
+    /\ contains h1 op.kp_log
+  ))
 
 val create_odh_package: (#key_length:(n:nat{n<=32})) -> (#key_type:(id -> Type0)) -> (kp:key_package key_length key_type) -> (oparam:odh_parameters{oparam.hash_length = key_length}) -> (rgn:erid) -> ST (odh_package #key_length #key_type kp oparam)
   (requires (fun h0 -> True))
@@ -116,10 +96,54 @@ val create_odh_package: (#key_length:(n:nat{n<=32})) -> (#key_type:(id -> Type0)
     modifies (Set.singleton rgn) h0 h1
     /\ extends op.rgn rgn
   ))
-let create_odh_package (#key_length:(n:nat{n<=32})) (#key_type:(id -> Type0)) (kp:key_package key_length key_type) (oparam:odh_parameters{oparam.hash_length = key_length}) (rgn:erid) =
-  let odh_rgn = new_region rgn in
-  let kp_log = MM.alloc #odh_rgn #key_package_log_key #(key_package_log_range key_type) #(key_package_log_inv key_type) in
-  ODH odh_rgn kp_log
+
+let dh_op_modified_regions (#key_length:(n:nat{n<=32})) (#key_type:(id -> Type0)) (#kp:key_package key_length key_type) (#oparam:odh_parameters{oparam.hash_length = key_length}) (op:odh_package kp oparam) (sh:share oparam) (exp:exponent oparam{exp.sh.raw_sh <> sh.raw_sh}) (h0:mem) : (GTot (Set.set rid)) =
+  let i = create_id sh exp.sh in
+  let both_honest = sh.h && exp.sh.h in
+  if both_honest && b then
+    match MM.sel (sel h0 op.kp_log) i with
+    | Some _ ->
+      Set.empty
+    | None ->
+        Set.singleton op.rgn
+  else
+    Set.empty
+
+let dh_op_log_change (#key_length:(n:nat{n<=32})) (#key_type:(id -> Type0)) (#kp:key_package key_length key_type) (#oparam:odh_parameters{oparam.hash_length = key_length}) (op:odh_package kp oparam) (sh:share oparam) (exp:exponent oparam{exp.sh.raw_sh <> sh.raw_sh}) (h0:mem) (h1:mem) =
+  let i = create_id sh exp.sh in
+  let both_honest = sh.h && exp.sh.h in
+  contains h0 op.kp_log
+  /\ ((both_honest /\ b) ==>
+      (MM.defined op.kp_log i h0 ==>
+        Some? (sel h1 op.kp_log i)
+        /\ (let k = Some?.v (sel h1 op.kp_log i) in
+          sel h1 op.kp_log == sel h0 op.kp_log
+        /\ witnessed (MM.contains op.kp_log i k)))
+      /\ (MM.fresh op.kp_log i h0 ==>
+          Some? (sel h1 op.kp_log i)
+          /\ (let k = Some?.v (sel h1 op.kp_log i) in
+          witnessed (MM.contains op.kp_log i k)
+          /\ sel h1 op.kp_log == MM.upd (sel h0 op.kp_log) i k))
+    )
+  /\ ((~both_honest \/ ~b) ==>
+      sel h1 op.kp_log == sel h0 op.kp_log)
+
+// Do we need/want this?
+let dh_op_functional_spec (#key_length:(n:nat{n<=32})) (#key_type:(id -> Type0)) (#kp:key_package key_length key_type) (#oparam:odh_parameters{oparam.hash_length = key_length}) (op:odh_package kp oparam) (sh:share oparam) (exp:exponent oparam{exp.sh.raw_sh <> sh.raw_sh}) (k:key_type (create_id sh exp.sh)) (h:mem) =
+  let i = create_id sh exp.sh in
+  let both_honest = sh.h && exp.sh.h in
+  ((both_honest) ==>
+    (b ==>
+      (Some? (MM.sel (sel h op.kp_log) i)
+      /\ k == Some?.v (MM.sel (sel h op.kp_log) i))) // If possible, indicate somehow that k was randomly drawn.
+    /\ (~b ==>
+      getGT kp i k == oparam.hash (oparam.exponentiate exp.raw_exp sh.raw_sh)
+      /\ hon kp i k = true)
+    )
+  /\ ((~both_honest) ==>
+      getGT kp i k == oparam.hash (oparam.exponentiate exp.raw_exp sh.raw_sh)
+      /\ hon kp i k = false)
+
 
 #set-options "--z3rlimit 300 --max_ifuel 2 --max_fuel 1"
 val dh_op: (#key_length:(n:nat{n<=32})) -> (#key_type:(id -> Type0)) -> (#kp:key_package key_length key_type) -> (#oparam:odh_parameters{oparam.hash_length = key_length}) -> op:odh_package kp oparam -> sh:share oparam -> exp:exponent oparam{exp.sh.raw_sh <> sh.raw_sh} -> ST (key_type (create_id sh exp.sh))
@@ -127,30 +151,18 @@ val dh_op: (#key_length:(n:nat{n<=32})) -> (#key_type:(id -> Type0)) -> (#kp:key
   (ensures (fun h0 k h1 ->
     let i = create_id sh exp.sh in
     let both_honest = sh.h && exp.sh.h in
-    ((both_honest /\ b) ==>
-      (MM.defined op.kp_log i h0 ==>
-        h0 == h1)
-      /\ (MM.fresh op.kp_log i h0 ==>
-        witnessed (MM.contains op.kp_log i k)
-        /\ sel h1 op.kp_log == MM.upd (sel h0 op.kp_log) i k
-        /\ modifies (Set.singleton op.rgn) h0 h1
-        ))
-    /\ ((~both_honest \/ ~b) ==>
-      h0 == h1)
-    /\ (modifies (Set.singleton op.rgn) h0 h1 \/ h0 == h1)
+    modifies (dh_op_modified_regions op sh exp h0) h0 h1
+    /\ dh_op_log_change op sh exp h0 h1
+   // /\ dh_op_functional_spec op sh exp k h1
+  /\ ((both_honest) ==>
+    (b ==>
+      (Some? (MM.sel (sel h1 op.kp_log) i)
+      /\ k == Some?.v (MM.sel (sel h1 op.kp_log) i)))
+    /\ (~b ==>
+      getGT kp i k == oparam.hash (oparam.exponentiate exp.raw_exp sh.raw_sh)
+      /\ hon kp i k = true)
+    ) // If possible, indicate somehow that k was randomly drawn.
+  /\ ((~both_honest) ==>
+      getGT kp i k == oparam.hash (oparam.exponentiate exp.raw_exp sh.raw_sh)
+      /\ hon kp i k = false)
   ))
-
-let dh_op #key_length #key_type #kp #oparam op sh exp =
-  let both_honest = sh.h && exp.sh.h in
-  let i = create_id sh exp.sh in
-  if both_honest && b then
-    (recall op.kp_log;
-    match MM.lookup op.kp_log i with
-    | None ->
-      let k = kp.gen i in
-      MM.extend op.kp_log i k;
-      k
-    | Some k -> k)
-  else
-    (recall op.kp_log;
-    kp.set i (oparam.hash (oparam.exponentiate exp.raw_exp sh.raw_sh)))
