secure_api/box/experimental_box/Box.AE_impl/Box.AE.fst
@@ -1,0 +1,84 @@
+module Box.AE
+
+open FStar.Set
+open FStar.Seq
+open FStar.HyperStack
+open FStar.HyperStack.ST
+
+open FStar.Endianness
+
+open Box.Plain
+
+module KEY = Box.Key
+module MM = FStar.Monotonic.Map
+
+// KEY Package definition
+
+let rec random_bytes n =
+  match n with
+  | 0 -> let l:lbytes 0 = createL [] in l
+  | _ -> append (createL [0x0buy]) (random_bytes (n-1))
+
+let hon #id #kl i k =
+ k.h
+
+let cget #id #kl i k =
+ k.raw
+
+let get #id #kl i k =
+ k.raw
+
+let getGT #id #kl i k =
+ k.raw
+
+let set #id #key_length i raw =
+  Key raw true
+
+let gen #id key_length i =
+ Key (random_bytes key_length) true
+
+let cset #id #key_length i raw =
+  Key raw false
+
+let create_ae_key_package id key_length =
+  KEY.create_key_package key_length (key key_length #id) (hon #id #key_length) (getGT #id #key_length) (cget #id #key_length) (get #id #key_length) (gen #id key_length) cset set
+
+let get_ap_rgn (#id:eqtype) (#key_length:(n:nat{n<=32})) (#kp:KEY.key_package #id key_length (key key_length #id)) (#aparams:ae_parameters{aparams.keylength = key_length}) (ap:ae_package #id #key_length kp aparams)= ap.rgn
+
+let recall_log (#id:eqtype) (#key_length:(n:nat{n<=32})) (#kp:KEY.key_package #id key_length (key key_length #id)) (#aparams:ae_parameters{aparams.keylength = key_length}) (ap:ae_package #id kp aparams) = recall ap.log
+
+let get_ap_log #id #key_length #kp #aparams ap = ap.log
+
+let create_ae_package (rgn:erid) (#id:eqtype) (#key_length:(n:nat{n<=32})) (kp:KEY.key_package #id key_length (key key_length #id)) (aparams:ae_parameters{aparams.keylength = key_length}) (b:bool) =
+  let rgn = new_region rgn in
+  let pp = PP b aparams.scheme.valid_plain_length in
+  let log = MM.alloc #rgn #(message_log_key id aparams) #(message_log_range #id pp aparams) #(message_log_inv #pp #aparams #id) in
+  AE #id #key_length #kp #aparams b pp rgn log
+
+let zero_bytes valid_length n = Seq.create n (UInt8.uint_to_t 0)
+
+#set-options "--max_fuel 1 --max_ifuel 1 --z3rlimit 300"
+let encrypt #id #i #key_length #kp #aparams ap k n p =
+  let c =
+    if KEY.(hon kp i k) && ap.b then
+      let p' = zero_bytes (ap.pp.valid_length) (length p) in
+      aparams.scheme.enc p' k.raw n
+    else
+      aparams.scheme.enc (repr #ap.pp kp k p) k.raw n
+  in
+  recall ap.log;
+  MM.extend ap.log (LOG_KEY i n c) p;
+  c
+
+let decrypt #id #i #key_length #kp #aparams ap k n c =
+  match KEY.(hon kp i k) && ap.b with
+  | true ->
+    (match MM.lookup ap.log (LOG_KEY i n c) with
+    | Some p ->
+       recall ap.log;
+       Some p
+    | None -> None)
+  | false ->
+    match aparams.scheme.dec c k.raw n with
+    | Some p -> Some (coerce #ap.pp kp k p)
+    | None -> None
