secure_api/box/experimental_box/Box.Key_impl/Box.Key.fst
@@ -1,0 +1,21 @@
+module Box.Key
+
+open FStar.Endianness
+
+// Definition KEY package
+let hon #id #key_length #key_type kp = kp.hon
+
+let getGT #id #key_length #key_type kp = kp.getGT
+
+let cget #id #key_length #key_type kp = kp.cget
+
+let get #id #key_length #key_type kp = kp.get
+
+let gen #id #key_length #key_type kp = kp.gen
+
+let cset #id #key_length #key_type kp = kp.cset
+
+let set #id #key_length #key_type kp = kp.set
+
+let create_key_package #id key_length key_type hon getGT cget get gen cset set =
+  KP hon getGT cget get gen cset set
