secure_api/box/experimental_box/Box.ODH_impl/Box.ODH.fst
@@ -1,0 +1,88 @@
+module Box.ODH
+
+open FStar.Set
+open FStar.Seq
+open FStar.HyperStack
+open FStar.HyperStack.ST
+
+open Box.Key
+
+open FStar.Endianness
+
+module MM = FStar.Monotonic.Map
+
+let rec random_bytes n =
+  match n with
+  | 0 -> let l:lbytes 0 = createL [] in l
+  | _ -> append (createL [0x0buy]) (random_bytes (n-1))
+
+let sh_hon #oparams sh = sh.h
+
+let exp_hon #oparams exp = exp.sh.h
+
+let get_exp_share #oparams e = e.sh
+
+let get_share_raw #oparams sh = sh.raw_sh
+
+let get_exponent_raw #oparams exp = exp.raw_exp
+
+let gen_dh (oparam:odh_parameters) =
+  let raw_exp = random_bytes oparam.exponent_length in
+  let raw_sh = oparam.exponentiate raw_exp oparam.generator in
+  let sh = SH raw_sh true in
+  EXP raw_exp sh
+
+let coerce_dh_sh  (oparam:odh_parameters) (raw_sh:lbytes oparam.share_length) =
+  SH raw_sh false
+
+let coerce_dh_exp  (oparam:odh_parameters) (raw_exp:lbytes oparam.exponent_length) =
+  let raw_sh = oparam.exponentiate raw_exp oparam.generator in
+  let sh = SH raw_sh false in
+  EXP raw_exp sh
+
+let create_id #oparam sh1 sh2 =
+  let int_sh1 = little_endian sh1.raw_sh in
+  let int_sh2 = little_endian sh2.raw_sh in
+  //let int_sh1 = int_of_bytes sh1.raw_sh in
+  //let int_sh2 = int_of_bytes sh2.raw_sh in
+  if int_sh1 < int_sh2 then
+    (sh1.raw_sh,sh2.raw_sh)
+  else
+    (sh2.raw_sh,sh1.raw_sh)
+
+let lemma_symmetric_id #oparam sh1 sh2 =
+  lemma_little_endian_bij sh1.raw_sh sh2.raw_sh
+
+let get_flag #key_length #key_type #kp #oparam op = op.b
+
+let get_op_rgn (#key_length:(n:nat{n<=32})) (#key_type:(id -> Type0)) (#kp:key_package key_length key_type) (#oparam:odh_parameters{oparam.hash_length = key_length}) (op:odh_package #key_length #key_type kp oparam) = op.rgn
+
+let get_op_log (#key_length:(n:nat{n<=32})) (#key_type:(id -> Type0)) (#kp:key_package key_length key_type) (#oparam:odh_parameters{oparam.hash_length = key_length}) (op:odh_package #key_length #key_type kp oparam) = op.kp_log
+
+let recall_op_log #key_length #key_type #kp #oparam op =
+  recall op.kp_log
+
+let create_odh_package (#key_length:(n:nat{n<=32})) (#key_type:(id -> Type0)) (kp:key_package key_length key_type) (oparam:odh_parameters{oparam.hash_length = key_length}) (rgn:erid) (b:bool) =
+  let odh_rgn = new_region rgn in
+  let kp_log = MM.alloc #odh_rgn #key_package_log_key #(key_package_log_range key_type) #(key_package_log_inv key_type) in
+  ODH odh_rgn b kp_log
+
+#set-options "--z3rlimit 300 --max_ifuel 2 --max_fuel 1"
+let dh_op #key_length #key_type #kp #oparam op sh exp =
+  let both_honest = sh.h && exp.sh.h in
+  let i = create_id sh exp.sh in
+  if both_honest then
+    if op.b then
+      (recall op.kp_log;
+      match MM.lookup op.kp_log i with
+      | None ->
+        let k = gen kp i in
+        MM.extend op.kp_log i k;
+        k
+      | Some k -> k)
+    else
+      (recall op.kp_log;
+      set kp i (oparam.hash (oparam.exponentiate exp.raw_exp sh.raw_sh)))
+  else
+    (recall op.kp_log;
+    cset kp i (oparam.hash (oparam.exponentiate exp.raw_exp sh.raw_sh)))
