secure_api/box/experimental_box/Box.ODH_proof/Box.Key.fsti
@@ -1,0 +1,44 @@
+module Box.Key
+
+open FStar.Endianness
+
+// Definition KEY package
+noeq abstract type key_package (#id:eqtype) (key_length:(n:nat{n<=32})) (key_type:(id  -> Type0)) =
+  | KP:
+  hon: (i:id -> key_type i -> bool) ->
+  getGT: (i:id -> k:key_type i -> GTot (lbytes key_length)) ->
+  cget: (i:id -> k:key_type i{hon i k = false} -> (raw:lbytes key_length{raw = getGT i k})) ->
+  get: (i:id -> k:key_type i -> (raw:lbytes key_length{raw = getGT i k})) ->
+  gen: (i:id -> k:key_type i{hon i k = true}) ->
+  cset: (i:id -> raw:lbytes key_length -> (k:key_type i{raw = getGT i k /\ hon i k = false})) ->
+  set: (i:id -> raw:lbytes key_length -> (k:key_type i{raw = getGT i k /\ hon i k = true})) ->
+  key_package #id key_length key_type
+
+val hon: (#id:eqtype) -> (#key_length:(n:nat{n<=32})) -> (#key_type:(id -> Type0)) -> kp:key_package #id key_length key_type -> (kp_hon:(i:id -> key_type i -> bool){kp_hon == kp.hon})
+
+val getGT: (#id:eqtype) -> (#key_length:(n:nat{n<=32})) -> (#key_type:(id -> Type0)) -> kp:key_package #id key_length key_type -> (kp_getGT:(i:id -> k:key_type i -> GTot (lbytes key_length)){kp_getGT == kp.getGT})
+
+val cget: (#id:eqtype) -> (#key_length:(n:nat{n<=32})) -> (#key_type:(id -> Type0)) -> kp:key_package #id key_length key_type -> (i:id -> k:key_type i{kp.hon i k = false} -> (raw:lbytes key_length{raw = kp.getGT i k}))
+
+val get: (#id:eqtype) -> (#key_length:(n:nat{n<=32})) -> (#key_type:(id -> Type0)) -> kp:key_package #id key_length key_type -> (i:id -> k:key_type i -> (raw:lbytes key_length{raw = kp.getGT i k}))
+
+#set-options "--z3rlimit 300 --max_ifuel 1 --max_fuel 0"
+val create_key_package:
+  (#id:eqtype) ->
+  (key_length:(n:nat{n<=32})) ->
+  (key_type:(id -> Type0)) ->
+  (param_hon:(i:id -> key_type i -> bool)) ->
+  (param_getGT: (i:id -> k:key_type i -> GTot (lbytes key_length))) ->
+  (param_cget: (i:id -> k:key_type i{param_hon i k = false} -> (raw:lbytes key_length{raw = param_getGT i k}))) ->
+  (param_get: (i:id -> k:key_type i -> (raw:lbytes key_length{raw = param_getGT i k}))) ->
+  (param_gen: (i:id -> k:key_type i{param_hon i k = true})) ->
+  (param_cset: (i:id -> raw:lbytes key_length -> (k:key_type i{raw = param_getGT i k /\ param_hon i k = false}))) ->
+  (param_set: (i:id -> raw:lbytes key_length -> (k:key_type i{raw = param_getGT i k /\ param_hon i k = true}))) ->
+  (kp:key_package #id key_length key_type{
+    param_hon == hon kp
+    /\ param_hon == kp.hon
+    /\ param_getGT == kp.getGT
+    /\ param_getGT == getGT kp
+    /\ param_cget == cget kp
+    /\ param_get == get kp
+  })
